Code/Preprocessing/Preprocessor.v
@@ -297,21 +297,15 @@ Definition to_rewriteRule
            (ar : members (BaseTerms X) -> ty (baseTypes X))
            (t : rawNe V F * rawNf V F)
   : option (rewriteRule ar)
-  := match t with
-     | pair t1 t2 =>
-       freeVars_to_con X
-       >>= fun C => check_functions_Ne X C ar t1
-       >>= fun t1 => rawNfToUtNe t1
-       >>= fun t1 => infer_to_tm C ar t1
-       >>= fun z =>
-             match z with
-             | (A , t1) =>
-               check_functions_Nf X C ar t2
-               >>= fun t2 => rawNfToUtNf t2
-               >>= fun t2 => check_to_tm C ar t2 A
-               >>= fun t2 => Some (make_rewrite C _ t1 t2)
-             end
-          end.
+  := freeVars_to_con X
+     >>= fun C => check_functions_Ne X C ar (fst t)
+     >>= fun t1 => rawNfToUtNe t1
+     >>= fun t1 => infer_to_tm C ar t1
+     >>= fun z =>
+           check_functions_Nf X C ar (snd t)
+           >>= fun t2 => rawNfToUtNf t2
+           >>= fun t2 => check_to_tm C ar t2 (projT1 z)
+           >>= fun t2 => Some (make_rewrite C _ (projT2 z) t2).
 
 Definition parsedAFS_to_afs
            {B V F : Type}
